added UNDEC for two counters Minsky machines with self-contained explanations

MM/mma_defs.v
@@ -38,13 +38,13 @@ Section Minsky_Machine_alternate.
 
   (* Minsky machine small step semantics *)
 
-  Inductive mm2_sss : mm_instr n -> mm_state n -> mm_state n -> Prop :=
-    | in_mm2_sss_inc   : forall i x v,                   INC x   // (i,v) -1> (1+i,v[(S (v#>x))/x])
-    | in_mm2_sss_dec_0 : forall i x k v,   v#>x = O   -> DEC x k // (i,v) -1> (1+i,v)
-    | in_mm2_sss_dec_1 : forall i x k v u, v#>x = S u -> DEC x k // (i,v) -1> (k,v[u/x])
-  where "i // s -1> t" := (mm2_sss i s t).
+  Inductive mma_sss : mm_instr n -> mm_state n -> mm_state n -> Prop :=
+    | in_mma_sss_inc   : forall i x v,                   INC x   // (i,v) -1> (1+i,v[(S (v#>x))/x])
+    | in_mma_sss_dec_0 : forall i x k v,   v#>x = O   -> DEC x k // (i,v) -1> (1+i,v)
+    | in_mma_sss_dec_1 : forall i x k v u, v#>x = S u -> DEC x k // (i,v) -1> (k,v[u/x])
+  where "i // s -1> t" := (mma_sss i s t).
 
-  Fact mm2_sss_fun i s t1 t2 : i // s -1> t1 -> i // s -1> t2 -> t1 = t2.
+  Fact mma_sss_fun i s t1 t2 : i // s -1> t1 -> i // s -1> t2 -> t1 = t2.
   Proof.
     intros []; subst.
     inversion 1; subst; auto.
@@ -55,7 +55,7 @@ Section Minsky_Machine_alternate.
     rewrite H in H6; inversion H6; subst; auto.
   Qed.
   
-  Fact mm2_sss_total ii s : { t | ii // s -1> t }.
+  Fact mma_sss_total ii s : { t | ii // s -1> t }.
   Proof.
     destruct s as (i,v).
     destruct ii as [ x | x j ]; [ | case_eq (v#>x); [ | intros k ]; intros E ].
@@ -64,25 +64,25 @@ Section Minsky_Machine_alternate.
     * exists (j,v[k/x]); constructor; auto.
   Qed.
   
-  Fact mm2_sss_INC_inv x i v j w : INC x // (i,v) -1> (j,w) -> j=1+i /\ w = v[(S (v#>x))/x].
+  Fact mma_sss_INC_inv x i v j w : INC x // (i,v) -1> (j,w) -> j=1+i /\ w = v[(S (v#>x))/x].
   Proof. inversion 1; subst; auto. Qed.
   
-  Fact mm2_sss_DEC0_inv x k i v j w : v#>x = O -> DEC x k // (i,v) -1> (j,w) -> j = 1+i /\ w = v.
+  Fact mma_sss_DEC0_inv x k i v j w : v#>x = O -> DEC x k // (i,v) -1> (j,w) -> j = 1+i /\ w = v.
   Proof. 
     intros H; inversion 1; subst; auto; rewrite H in H2; try discriminate.
   Qed.
   
-  Fact mm2_sss_DEC1_inv x k u i v j w : v#>x = S u -> DEC x k // (i,v) -1> (j,w) -> j=k /\ w = v[u/x].
+  Fact mma_sss_DEC1_inv x k u i v j w : v#>x = S u -> DEC x k // (i,v) -1> (j,w) -> j=k /\ w = v[u/x].
   Proof. 
     intros H; inversion 1; subst; auto; rewrite H in H2; try discriminate.
     inversion H2; subst; auto.
   Qed.
 
-  Notation "P // s -[ k ]-> t" := (sss_steps mm2_sss P k s t).
-  Notation "P // s -+> t" := (sss_progress mm2_sss P s t).
-  Notation "P // s ->> t" := (sss_compute mm2_sss P s t).
+  Notation "P // s -[ k ]-> t" := (sss_steps mma_sss P k s t).
+  Notation "P // s -+> t" := (sss_progress mma_sss P s t).
+  Notation "P // s ->> t" := (sss_compute mma_sss P s t).
   
-  Fact mm2_sss_progress_INC P i x v st :
+  Fact mma_sss_progress_INC P i x v st :
          (i,INC x::nil) <sc P
       -> P // (1+i,v[(S (v#>x))/x]) ->> st
       -> P // (i,v) -+> st.
@@ -96,10 +96,10 @@ Section Minsky_Machine_alternate.
     constructor; auto.
   Qed.
   
-  Corollary mm2_sss_compute_INC P i x v st : (i,INC x::nil) <sc P -> P // (1+i,v[(S (v#>x))/x]) ->> st -> P // (i,v) ->> st.
-  Proof. intros; apply sss_progress_compute; eapply mm2_sss_progress_INC; eauto. Qed.
+  Corollary mma_sss_compute_INC P i x v st : (i,INC x::nil) <sc P -> P // (1+i,v[(S (v#>x))/x]) ->> st -> P // (i,v) ->> st.
+  Proof. intros; apply sss_progress_compute; eapply mma_sss_progress_INC; eauto. Qed.
   
-  Fact mm2_sss_progress_DEC_0 P i x k v st :
+  Fact mma_sss_progress_DEC_0 P i x k v st :
          (i,DEC x k::nil) <sc P
       -> v#>x = O 
       -> P // (1+i,v) ->> st
@@ -114,10 +114,10 @@ Section Minsky_Machine_alternate.
     constructor; auto.
   Qed.
   
-  Corollary mm2_sss_compute_DEC_0 P i x k v st : (i,DEC x k::nil) <sc P -> v#>x = O -> P // (1+i,v) ->> st -> P // (i,v) ->> st.
-  Proof. intros; apply sss_progress_compute; eapply mm2_sss_progress_DEC_0; eauto. Qed.
+  Corollary mma_sss_compute_DEC_0 P i x k v st : (i,DEC x k::nil) <sc P -> v#>x = O -> P // (1+i,v) ->> st -> P // (i,v) ->> st.
+  Proof. intros; apply sss_progress_compute; eapply mma_sss_progress_DEC_0; eauto. Qed.
   
-  Fact mm2_sss_progress_DEC_S P i x k v u st :
+  Fact mma_sss_progress_DEC_S P i x k v u st :
          (i,DEC x k::nil) <sc P
       -> v#>x = S u 
       -> P // (k,v[u/x]) ->> st
@@ -132,10 +132,10 @@ Section Minsky_Machine_alternate.
     constructor; auto.
   Qed.
   
-  Corollary mm2_sss_compute_DEC_S P i x k v u st : (i,DEC x k::nil) <sc P -> v#>x = S u -> P // (k,v[u/x]) ->> st -> P // (i,v) ->> st.
-  Proof. intros; apply sss_progress_compute; eapply mm2_sss_progress_DEC_S; eauto. Qed.
+  Corollary mma_sss_compute_DEC_S P i x k v u st : (i,DEC x k::nil) <sc P -> v#>x = S u -> P // (k,v[u/x]) ->> st -> P // (i,v) ->> st.
+  Proof. intros; apply sss_progress_compute; eapply mma_sss_progress_DEC_S; eauto. Qed.
   
-  Fact mm2_sss_steps_INC_inv k P i x v st :
+  Fact mma_sss_steps_INC_inv k P i x v st :
          (i,INC x::nil) <sc P
       -> k <> 0
       -> P // (i,v) -[k]-> st
@@ -151,7 +151,7 @@ Section Minsky_Machine_alternate.
     inversion H4; subst; auto.
   Qed.
   
-  Fact mm2_sss_steps_DEC_0_inv k P i x p v st :
+  Fact mma_sss_steps_DEC_0_inv k P i x p v st :
          (i,DEC x p::nil) <sc P
       -> k <> 0
       -> v#>x = 0
@@ -169,7 +169,7 @@ Section Minsky_Machine_alternate.
     rewrite H3 in H9; discriminate.
   Qed.
   
-  Fact mm2_sss_steps_DEC_1_inv k P i x p v u st :
+  Fact mma_sss_steps_DEC_1_inv k P i x p v u st :
          (i,DEC x p::nil) <sc P
       -> k <> 0
       -> v#>x = S u
@@ -190,29 +190,33 @@ Section Minsky_Machine_alternate.
 
 End Minsky_Machine_alternate.
 
-Local Notation "P // s -[ k ]-> t" := (sss_steps (@mm2_sss _) P k s t).
-Local Notation "P // s -+> t" := (sss_progress (@mm2_sss _) P s t).
-Local Notation "P // s ->> t" := (sss_compute (@mm2_sss _) P s t).
+Local Notation "P // s -+> t" := (sss_progress (@mma_sss _) P s t).
+Local Notation "P // s ->> t" := (sss_compute (@mma_sss _) P s t).
+Local Notation "P // s ↓" := (sss_terminates (@mma_sss _) P s). 
 
-Tactic Notation "mm2" "sss" "INC" "with" uconstr(a) := 
+Tactic Notation "mma" "sss" "INC" "with" uconstr(a) := 
   match goal with
-    | |- _ // _ -+> _ => apply mm2_sss_progress_INC with (x := a)
-    | |- _ // _ ->> _ => apply mm2_sss_compute_INC with (x := a)
+    | |- _ // _ -+> _ => apply mma_sss_progress_INC with (x := a)
+    | |- _ // _ ->> _ => apply mma_sss_compute_INC with (x := a)
   end; auto.
 
-Tactic Notation "mm2" "sss" "DEC" "0" "with" uconstr(a) uconstr(b) := 
+Tactic Notation "mma" "sss" "DEC" "0" "with" uconstr(a) uconstr(b) := 
   match goal with
-    | |- _ // _ -+> _ => apply mm2_sss_progress_DEC_0 with (x := a) (k := b)
-    | |- _ // _ ->> _ => apply mm2_sss_compute_DEC_0 with (x := a) (k := b)
+    | |- _ // _ -+> _ => apply mma_sss_progress_DEC_0 with (x := a) (k := b)
+    | |- _ // _ ->> _ => apply mma_sss_compute_DEC_0 with (x := a) (k := b)
   end; auto.
 
-Tactic Notation "mm2" "sss" "DEC" "S" "with" uconstr(a) uconstr(b) uconstr(c) := 
+Tactic Notation "mma" "sss" "DEC" "S" "with" uconstr(a) uconstr(b) uconstr(c) := 
   match goal with
-    | |- _ // _ -+> _ => apply mm2_sss_progress_DEC_S with (x := a) (k := b) (u := c)
-    | |- _ // _ ->> _ => apply mm2_sss_compute_DEC_S with (x := a) (k := b) (u := c)
+    | |- _ // _ -+> _ => apply mma_sss_progress_DEC_S with (x := a) (k := b) (u := c)
+    | |- _ // _ ->> _ => apply mma_sss_compute_DEC_S with (x := a) (k := b) (u := c)
   end; auto.
     
-Tactic Notation "mm2" "sss" "stop" := exists 0; apply sss_steps_0; auto.
+Tactic Notation "mma" "sss" "stop" := exists 0; apply sss_steps_0; auto.
+
+Definition MMA2_PROBLEM := (list (mm_instr 2) * vec nat 2)%type.
+Definition MMA2_HALTING (P : MMA2_PROBLEM) := (1,fst P) // (1,snd P) ↓.
+
 
 
 
