MM/mma_utils.v
@@ -10,7 +10,7 @@
 Require Import List Arith Omega.
 
 Require Import utils pos vec gcd.
-Require Import subcode sss mm2_defs.
+Require Import subcode sss mma_defs.
 
 Set Implicit Arguments.
 
@@ -19,10 +19,10 @@ Tactic Notation "rew" "length" := autorewrite with length_db.
 Local Notation "e #> x" := (vec_pos e x).
 Local Notation "e [ v / x ]" := (vec_change e x v).
 
-Local Notation "P // s -[ k ]-> t" := (sss_steps (@mm2_sss _) P k s t).
-Local Notation "P // s -+> t" := (sss_progress (@mm2_sss _) P s t).
-Local Notation "P // s ->> t" := (sss_compute (@mm2_sss _) P s t).
-Local Notation "P // s ↓" := (sss_terminates (@mm2_sss _) P s). 
+Local Notation "P // s -[ k ]-> t" := (sss_steps (@mma_sss _) P k s t).
+Local Notation "P // s -+> t" := (sss_progress (@mma_sss _) P s t).
+Local Notation "P // s ->> t" := (sss_compute (@mma_sss _) P s t).
+Local Notation "P // s ↓" := (sss_terminates (@mma_sss _) P s). 
 
 (** Utils for FRACTRAN with two counter *)
 
@@ -34,124 +34,124 @@ Section Minsky_Machine_alt_utils.
 
   Hint Resolve subcode_refl.
 
-  Section mm2_null.
+  Section mma_null.
 
     (* Empty oone register/counter *)
 
     Variable (dst : pos n).
 
-    Definition mm2_null i := DEC dst i :: nil.
+    Definition mma_null i := DEC dst i :: nil.
 
-    Fact mm2_null_length i : length (mm2_null i) = 1.
+    Fact mma_null_length i : length (mma_null i) = 1.
     Proof. auto. Qed.
     
-    Let mm2_null_spec i k v w : v#>dst = k 
+    Let mma_null_spec i k v w : v#>dst = k 
                              -> w = v[0/dst]
-                             -> (i,mm2_null i) // (i,v) -+> (1+i,w).
+                             -> (i,mma_null i) // (i,v) -+> (1+i,w).
     Proof.
-      unfold mm2_null.
+      unfold mma_null.
       revert v w.
       induction k as [ | k IHk ]; intros v w H1 H2; subst w.
-      + mm2 sss DEC 0 with dst i.
-        mm2 sss stop; f_equal.
+      + mma sss DEC 0 with dst i.
+        mma sss stop; f_equal.
         apply vec_pos_ext; intros z; dest z dst.
-      + mm2 sss DEC S with dst i k.
+      + mma sss DEC S with dst i k.
         apply sss_progress_compute.
         apply IHk; rew vec.
     Qed.
 
-    Fact mm2_null_progress i v st : 
+    Fact mma_null_progress i v st : 
              st = (1+i,v[0/dst])
-          -> (i,mm2_null i) // (i,v) -+> st.
+          -> (i,mma_null i) // (i,v) -+> st.
     Proof.
       intros; subst.
-      apply mm2_null_spec with (1 := eq_refl); auto.
+      apply mma_null_spec with (1 := eq_refl); auto.
     Qed.
 
-  End mm2_null.
+  End mma_null.
 
-  Hint Rewrite mm2_null_length : length_db.
+  Hint Rewrite mma_null_length : length_db.
 
-  Section mm2_transfert.
+  Section mma_transfert.
 
     (* Added the content of src to dst while emptying src *)
 
     Variables (src dst : pos n) (Hsd : src <> dst).
 
-    Definition mm2_transfert i := INC dst :: DEC src i :: DEC dst (3+i) :: nil.
+    Definition mma_transfert i := INC dst :: DEC src i :: DEC dst (3+i) :: nil.
 
-    Fact mm2_transfert_length i : length (mm2_transfert i) = 3.
+    Fact mma_transfert_length i : length (mma_transfert i) = 3.
     Proof. reflexivity. Qed.
 
-    Let mm2_transfert_spec i v w k x :  v#>src = k
+    Let mma_transfert_spec i v w k x :  v#>src = k
                                      -> v#>dst = x
                                      -> w = v[0/src][(1+k+x)/dst]
-                                     -> (i,mm2_transfert i) // (i,v) -+> (2+i,w).
+                                     -> (i,mma_transfert i) // (i,v) -+> (2+i,w).
     Proof.
-      unfold mm2_transfert.
+      unfold mma_transfert.
       revert v w x.
       induction k as [ | k IHk ]; intros v w x H1 H2 H3; subst w.
-      + mm2 sss INC with dst.
-        mm2 sss DEC 0 with src i; rew vec.
-        mm2 sss stop; f_equal; auto.
+      + mma sss INC with dst.
+        mma sss DEC 0 with src i; rew vec.
+        mma sss stop; f_equal; auto.
         apply vec_pos_ext; intros z; dest z dst; dest z src.
-      + mm2 sss INC with dst.
-        mm2 sss DEC S with src i k; rew vec.
+      + mma sss INC with dst.
+        mma sss DEC S with src i k; rew vec.
         apply sss_progress_compute, IHk with (x := 1+x); rew vec.
         apply vec_pos_ext; intros p.
         dest p dst; try omega; dest p src.
     Qed.
 
-    Fact mm2_transfert_progress i v st : 
+    Fact mma_transfert_progress i v st : 
            st = (3+i,v[0/src][((v#>src)+(v#>dst))/dst])
-        -> (i,mm2_transfert i) // (i,v) -+> st.
+        -> (i,mma_transfert i) // (i,v) -+> st.
     Proof.
       intros ?; subst.
       apply sss_progress_trans with (2+i, v[0/src][(1+(v#>src)+(v#>dst))/dst]).
-      + apply mm2_transfert_spec with (1 := eq_refl) (2 := eq_refl); auto.
-      + unfold mm2_transfert.
-        mm2 sss DEC S with dst (3+i) ((v#>src)+(v#>dst)); rew vec.
-        mm2 sss stop.
+      + apply mma_transfert_spec with (1 := eq_refl) (2 := eq_refl); auto.
+      + unfold mma_transfert.
+        mma sss DEC S with dst (3+i) ((v#>src)+(v#>dst)); rew vec.
+        mma sss stop.
     Qed.
 
-  End mm2_transfert.
+  End mma_transfert.
 
-  Hint Rewrite mm2_transfert_length : length_db.
+  Hint Rewrite mma_transfert_length : length_db.
 
-  Section mm2_incs.
+  Section mma_incs.
 
     (* Add a constant value k to dst *)
 
     Variable (dst : pos n).
 
-    Fixpoint mm2_incs k := 
+    Fixpoint mma_incs k := 
       match k with 
         | 0   => nil
-        | S k => INC dst :: mm2_incs k
+        | S k => INC dst :: mma_incs k
       end.
 
-    Fact mm2_incs_length k : length (mm2_incs k) = k.
+    Fact mma_incs_length k : length (mma_incs k) = k.
     Proof. induction k; simpl; f_equal; auto. Qed.
 
-    Fact mm2_incs_compute k i v st :
+    Fact mma_incs_compute k i v st :
              st = (k+i,v[(k+(v#>dst))/dst])
-          -> (i,mm2_incs k) // (i,v) ->> st.
+          -> (i,mma_incs k) // (i,v) ->> st.
     Proof.
       revert i v st; induction k as [ | k IHk ]; intros i v st ?; subst.
-      + mm2 sss stop; f_equal; auto.
+      + mma sss stop; f_equal; auto.
         apply vec_pos_ext; intros p; dest p dst.
-      + simpl; mm2 sss INC with dst.
-        apply subcode_sss_compute with (P := (1+i,mm2_incs k)); auto.
+      + simpl; mma sss INC with dst.
+        apply subcode_sss_compute with (P := (1+i,mma_incs k)); auto.
         { subcode_tac; rewrite <- app_nil_end; auto. }
         apply IHk; f_equal; try omega.
         apply vec_pos_ext; intros p; dest p dst.
     Qed.
 
-  End mm2_incs.
+  End mma_incs.
 
-  Section mm2_decs.
+  Section mma_decs.
 
-    (* "mm2_dec dst p q k" at i 
+    (* "mma_dec dst p q k" at i 
 
         removes constant k to dst:
 
@@ -162,313 +162,313 @@ Section Minsky_Machine_alt_utils.
 
     Variable (dst : pos n) (p q : nat).
 
-    Fixpoint mm2_decs k i := 
+    Fixpoint mma_decs k i := 
       match k with 
         | 0   => INC dst :: DEC dst p :: nil
-        | S k => DEC dst (3+i) :: INC dst :: DEC dst q :: mm2_decs k (3+i)
+        | S k => DEC dst (3+i) :: INC dst :: DEC dst q :: mma_decs k (3+i)
       end.
 
-    Fact mm2_decs_length k i : length (mm2_decs k i) = 2+3*k.
+    Fact mma_decs_length k i : length (mma_decs k i) = 2+3*k.
     Proof.
       revert i; induction k as [ | ? IHk ]; intros i; simpl; auto.
       rewrite IHk; omega.
     Qed.
 
-    Let mm2_decs_spec_lt k i v w : 
+    Let mma_decs_spec_lt k i v w : 
             v#>dst < k 
          -> w = v[0/dst]
-         -> (i,mm2_decs k i) // (i,v) -+> (q,w).
+         -> (i,mma_decs k i) // (i,v) -+> (q,w).
     Proof.
       revert i v w; induction k as [ | k IHk ]; intros i v w H1 ?; subst w.
       + omega.
-      + unfold mm2_decs; fold mm2_decs.
+      + unfold mma_decs; fold mma_decs.
         case_eq (v#>dst).
         * intros H2.
-          mm2 sss DEC 0 with dst (3+i).
-          mm2 sss INC with dst.
-          mm2 sss DEC S with dst q (v#>dst); rew vec.
-          mm2 sss stop; f_equal.
+          mma sss DEC 0 with dst (3+i).
+          mma sss INC with dst.
+          mma sss DEC S with dst q (v#>dst); rew vec.
+          mma sss stop; f_equal.
           apply vec_pos_ext; intros x; dest x dst.
         * intros d Hd.
-          mm2 sss DEC S with dst (3+i) d.
-          apply subcode_sss_compute with (P := (3+i,mm2_decs k (3+i))); auto.
+          mma sss DEC S with dst (3+i) d.
+          apply subcode_sss_compute with (P := (3+i,mma_decs k (3+i))); auto.
           { subcode_tac; rewrite <- app_nil_end; auto. }
           apply sss_progress_compute, IHk; rew vec; try omega.
     Qed.
 
-    Let mm2_decs_spec_le k i v w : 
+    Let mma_decs_spec_le k i v w : 
             k <= v#>dst 
          -> w = v[((v#>dst)-k)/dst]
-         -> (i,mm2_decs k i) // (i,v) -+> (p,w).
+         -> (i,mma_decs k i) // (i,v) -+> (p,w).
     Proof.
       revert i v w; induction k as [ | k IHk ]; intros i v w H1 ?; subst w.
       + simpl.
-        mm2 sss INC with dst.
-        mm2 sss DEC S with dst p (v#>dst); rew vec.
-        mm2 sss stop; f_equal.
+        mma sss INC with dst.
+        mma sss DEC S with dst p (v#>dst); rew vec.
+        mma sss stop; f_equal.
         apply vec_pos_ext; intros x; dest x dst; try omega.
-      + unfold mm2_decs; fold mm2_decs.
-        mm2 sss DEC S with dst (3+i) ((v#>dst) - 1); try omega.
-        apply subcode_sss_compute with (P := (3+i,mm2_decs k (3+i))); auto.
+      + unfold mma_decs; fold mma_decs.
+        mma sss DEC S with dst (3+i) ((v#>dst) - 1); try omega.
+        apply subcode_sss_compute with (P := (3+i,mma_decs k (3+i))); auto.
         { subcode_tac; rewrite <- app_nil_end; auto. }
         apply sss_progress_compute, IHk; rew vec; try omega.
         apply vec_pos_ext; intros x; dest x dst; omega.
     Qed.
 
-    Fact mm2_decs_lt_progress k i v st :
+    Fact mma_decs_lt_progress k i v st :
              v#>dst < k 
           -> st = (q,v[0/dst])
-          -> (i,mm2_decs k i) // (i,v) -+> st.
+          -> (i,mma_decs k i) // (i,v) -+> st.
     Proof.
       intros H1 ?; subst st.
-      apply mm2_decs_spec_lt; auto.
+      apply mma_decs_spec_lt; auto.
     Qed.
 
-    Fact mm2_decs_le_progress k i v st :
+    Fact mma_decs_le_progress k i v st :
              k <= v#>dst 
           -> st = (p,v[((v#>dst)-k)/dst])
-          -> (i,mm2_decs k i) // (i,v) -+> st.
+          -> (i,mma_decs k i) // (i,v) -+> st.
     Proof.
       intros H1 ?; subst st.
-      apply mm2_decs_spec_le; auto.
+      apply mma_decs_spec_le; auto.
     Qed.
 
-  End mm2_decs.
+  End mma_decs.
 
-  Section mm2_decs_copy.
+  Section mma_decs_copy.
 
-    (* Same as mm2_decs except that the quantity
+    (* Same as mma_decs except that the quantity
        removed from dst is transfered into tmp *)
 
     Variable (dst tmp : pos n) (Hdt : dst <> tmp) (p q : nat).
 
-    Fixpoint mm2_decs_copy k i := 
+    Fixpoint mma_decs_copy k i := 
       match k with 
         | 0   => INC dst :: DEC dst p :: nil
-        | S k => DEC dst (3+i) :: INC dst :: DEC dst q :: INC tmp :: mm2_decs_copy k (4+i)
+        | S k => DEC dst (3+i) :: INC dst :: DEC dst q :: INC tmp :: mma_decs_copy k (4+i)
       end.
 
-    Fact mm2_decs_copy_length k i : length (mm2_decs_copy k i) = 2+4*k.
+    Fact mma_decs_copy_length k i : length (mma_decs_copy k i) = 2+4*k.
     Proof.
       revert i; induction k as [ | ? IHk ]; intros i; simpl; auto.
       rewrite IHk; omega.
     Qed.
 
-    Let mm2_decs_copy_spec_lt k i v w : 
+    Let mma_decs_copy_spec_lt k i v w : 
             v#>dst < k 
          -> w = v[0/dst][((v#>dst)+(v#>tmp))/tmp]
-         -> (i,mm2_decs_copy k i) // (i,v) -+> (q,w).
+         -> (i,mma_decs_copy k i) // (i,v) -+> (q,w).
     Proof.
       revert i v w; induction k as [ | k IHk ]; intros i v w H1 ?; subst w.
       + omega.
-      + unfold mm2_decs_copy; fold mm2_decs_copy.
+      + unfold mma_decs_copy; fold mma_decs_copy.
         case_eq (v#>dst).
         * intros H2.
-          mm2 sss DEC 0 with dst (3+i).
-          mm2 sss INC with dst.
-          mm2 sss DEC S with dst q (v#>dst); rew vec.
-          mm2 sss stop; f_equal.
+          mma sss DEC 0 with dst (3+i).
+          mma sss INC with dst.
+          mma sss DEC S with dst q (v#>dst); rew vec.
+          mma sss stop; f_equal.
           apply vec_pos_ext; intros x; dest x tmp; dest x dst.
         * intros d Hd.
-          mm2 sss DEC S with dst (3+i) d.
-          mm2 sss INC with tmp.
-          apply subcode_sss_compute with (P := (4+i,mm2_decs_copy k (4+i))); auto.
+          mma sss DEC S with dst (3+i) d.
+          mma sss INC with tmp.
+          apply subcode_sss_compute with (P := (4+i,mma_decs_copy k (4+i))); auto.
           { subcode_tac; rewrite <- app_nil_end; auto. }
           apply sss_progress_compute; rewrite plus_assoc.
           apply IHk; rew vec; try omega.
           apply vec_pos_ext; intros x; dest x tmp; try omega; dest x dst.
     Qed.
 
-    Let mm2_decs_copy_spec_le k i v w : 
+    Let mma_decs_copy_spec_le k i v w : 
             k <= v#>dst 
          -> w = v[((v#>dst)-k)/dst][(k+(v#>tmp))/tmp]
-         -> (i,mm2_decs_copy k i) // (i,v) -+> (p,w).
+         -> (i,mma_decs_copy k i) // (i,v) -+> (p,w).
     Proof.
       revert i v w; induction k as [ | k IHk ]; intros i v w H1 ?; subst w.
       + simpl.
-        mm2 sss INC with dst.
-        mm2 sss DEC S with dst p (v#>dst); rew vec.
-        mm2 sss stop; f_equal.
+        mma sss INC with dst.
+        mma sss DEC S with dst p (v#>dst); rew vec.
+        mma sss stop; f_equal.
         apply vec_pos_ext; intros x; dest x dst; try omega; dest x tmp.
-      + unfold mm2_decs_copy; fold mm2_decs_copy.
-        mm2 sss DEC S with dst (3+i) ((v#>dst) - 1); try omega.
-        mm2 sss INC with tmp.
-        apply subcode_sss_compute with (P := (4+i,mm2_decs_copy k (4+i))); auto.
+      + unfold mma_decs_copy; fold mma_decs_copy.
+        mma sss DEC S with dst (3+i) ((v#>dst) - 1); try omega.
+        mma sss INC with tmp.
+        apply subcode_sss_compute with (P := (4+i,mma_decs_copy k (4+i))); auto.
         { subcode_tac; rewrite <- app_nil_end; auto. }
         apply sss_progress_compute, IHk; rew vec; try omega.
         apply vec_pos_ext; intros x; dest x tmp; try omega; dest x dst; omega.
     Qed.
 
-    Fact mm2_decs_copy_lt_progress k i v st :
+    Fact mma_decs_copy_lt_progress k i v st :
              v#>dst < k 
           -> st = (q,v[0/dst][((v#>dst)+(v#>tmp))/tmp])
-          -> (i,mm2_decs_copy k i) // (i,v) -+> st.
+          -> (i,mma_decs_copy k i) // (i,v) -+> st.
     Proof.
       intros H1 ?; subst st.
-      apply mm2_decs_copy_spec_lt; auto.
+      apply mma_decs_copy_spec_lt; auto.
     Qed.
 
-    Fact mm2_decs_copy_le_progress k i v st :
+    Fact mma_decs_copy_le_progress k i v st :
              k <= v#>dst 
           -> st = (p,v[((v#>dst)-k)/dst][(k+(v#>tmp))/tmp])
-          -> (i,mm2_decs_copy k i) // (i,v) -+> st.
+          -> (i,mma_decs_copy k i) // (i,v) -+> st.
     Proof.
       intros H1 ?; subst st.
-      apply mm2_decs_copy_spec_le; auto.
+      apply mma_decs_copy_spec_le; auto.
     Qed.
 
-  End mm2_decs_copy.
+  End mma_decs_copy.
 
-  Hint Rewrite mm2_incs_length mm2_decs_copy_length : length_db.
+  Hint Rewrite mma_incs_length mma_decs_copy_length : length_db.
  
-  Section mm2_mult_cst.
+  Section mma_mult_cst.
 
     (* dst <- k*src+dst *)
 
     Variable (src dst : pos n) (Hsd : src <> dst) (k i : nat).
 
-    Definition mm2_mult_cst :=
+    Definition mma_mult_cst :=
            DEC src (3+i) :: INC src :: DEC src (5+k+i) 
-        :: mm2_incs dst (S k) ++ DEC dst i :: nil. 
+        :: mma_incs dst (S k) ++ DEC dst i :: nil. 
 
-    Fact mm2_mult_cst_length : length mm2_mult_cst = 5+k.
-    Proof. unfold mm2_mult_cst; rew length; omega. Qed.
+    Fact mma_mult_cst_length : length mma_mult_cst = 5+k.
+    Proof. unfold mma_mult_cst; rew length; omega. Qed.
 
-    Let mm2_mult_cst_spec x v st :
+    Let mma_mult_cst_spec x v st :
              v#>src = x
           -> st = (5+k+i,v[0/src][(x*k+(v#>dst))/dst])
-          -> (i,mm2_mult_cst) // (i,v) -+> st.
+          -> (i,mma_mult_cst) // (i,v) -+> st.
     Proof.
-      unfold mm2_mult_cst.
+      unfold mma_mult_cst.
       revert v st; induction x as [ | x IHx ]; intros v st Hv ?; subst.
-      + mm2 sss DEC 0 with src (3+i).
-        mm2 sss INC with src.
-        mm2 sss DEC S with src (5+k+i) 0; rew vec.
-        mm2 sss stop; f_equal.
+      + mma sss DEC 0 with src (3+i).
+        mma sss INC with src.
+        mma sss DEC S with src (5+k+i) 0; rew vec.
+        mma sss stop; f_equal.
         apply vec_pos_ext; intros y; dest y dst; omega.
-      + mm2 sss DEC S with src (3+i) x.
+      + mma sss DEC S with src (3+i) x.
         apply sss_compute_trans with (4+k+i,v[x/src][(S k+(v#>dst))/dst]).
-        * apply subcode_sss_compute with (P := (3+i,mm2_incs dst (S k))); auto.
-          apply mm2_incs_compute; f_equal; try omega.
+        * apply subcode_sss_compute with (P := (3+i,mma_incs dst (S k))); auto.
+          apply mma_incs_compute; f_equal; try omega.
           apply vec_pos_ext; intros y; dest y dst; omega.
-        * mm2 sss DEC S with dst i (k+(v#>dst)); rew vec.
+        * mma sss DEC S with dst i (k+(v#>dst)); rew vec.
           apply sss_progress_compute, IHx; rew vec; f_equal.
           apply vec_pos_ext; intros y; dest y dst; try ring.
           dest y src.
     Qed.
 
-    Fact mm2_mult_cst_progress v st :
+    Fact mma_mult_cst_progress v st :
              st = (5+k+i,v[0/src][(k*(v#>src)+(v#>dst))/dst])
-          -> (i,mm2_mult_cst) // (i,v) -+> st.
+          -> (i,mma_mult_cst) // (i,v) -+> st.
     Proof.
       intros ?; subst.
-      apply mm2_mult_cst_spec with (1 := eq_refl); do 2 f_equal.
+      apply mma_mult_cst_spec with (1 := eq_refl); do 2 f_equal.
       ring.
     Qed.
 
-  End mm2_mult_cst.
+  End mma_mult_cst.
 
-  Hint Rewrite mm2_mult_cst_length : length_db.
+  Hint Rewrite mma_mult_cst_length : length_db.
   
-  Section mm2_mod_cst.
+  Section mma_mod_cst.
 
     (* test whether k divides src and transfer of src into dst *)
 
     Variable (src dst : pos n) (Hsd : src <> dst) (p q k i : nat).
 
-    Definition mm2_mod_cst :=
+    Definition mma_mod_cst :=
             DEC src (3+i)
          :: INC dst
          :: DEC dst p
          :: INC src
-         :: mm2_decs_copy src dst i q k (4+i).
+         :: mma_decs_copy src dst i q k (4+i).
 
-    Fact mm2_mod_cst_length : length mm2_mod_cst = 6+4*k.
-    Proof. unfold mm2_mod_cst; rew length; omega. Qed.
+    Fact mma_mod_cst_length : length mma_mod_cst = 6+4*k.
+    Proof. unfold mma_mod_cst; rew length; omega. Qed.
 
     (* This is of no use when k = 0 *)
 
     Hypothesis (Hk : 0 < k).
 
-    Let mm2_mod_cst_spec_0 v :
+    Let mma_mod_cst_spec_0 v :
            v#>src = 0
-        -> (i,mm2_mod_cst) // (i,v) -+> (p,v).
+        -> (i,mma_mod_cst) // (i,v) -+> (p,v).
     Proof.
-      intros H; unfold mm2_mod_cst.
-      mm2 sss DEC 0 with src (3+i).
-      mm2 sss INC with dst.
-      mm2 sss DEC S with dst p (v#>dst); rew vec.
-      mm2 sss stop.
+      intros H; unfold mma_mod_cst.
+      mma sss DEC 0 with src (3+i).
+      mma sss INC with dst.
+      mma sss DEC S with dst p (v#>dst); rew vec.
+      mma sss stop.
     Qed.
 
-    Let mm2_mod_cst_spec_1 a b v w :
+    Let mma_mod_cst_spec_1 a b v w :
            v#>src = a*k+b
         -> w = v[b/src][(a*k+(v#>dst))/dst]
-        -> (i,mm2_mod_cst) // (i,v) ->> (i,w).
+        -> (i,mma_mod_cst) // (i,v) ->> (i,w).
     Proof.
       revert v w; induction a as [ | a IHa ]; intros v w H1 H2; subst w.
-      + mm2 sss stop; f_equal.
+      + mma sss stop; f_equal.
         simpl in H1; rewrite <- H1; simpl; rew vec.
-      + unfold mm2_mod_cst.
-        mm2 sss DEC S with src (3+i) (S a*k+b-1).
+      + unfold mma_mod_cst.
+        mma sss DEC S with src (3+i) (S a*k+b-1).
         { rewrite H1; simpl; generalize (a*k); intro; omega. }
-        mm2 sss INC with src.
+        mma sss INC with src.
         apply sss_compute_trans with (i, v[(a*k+b)/src][(k+(v#>dst))/dst]).
-        * apply subcode_sss_compute with (P := (4+i,mm2_decs_copy src dst i q k (4+i))); auto.
+        * apply subcode_sss_compute with (P := (4+i,mma_decs_copy src dst i q k (4+i))); auto.
           { subcode_tac; rewrite <- app_nil_end; auto. }
-          apply sss_progress_compute, mm2_decs_copy_le_progress; auto; rew vec.
+          apply sss_progress_compute, mma_decs_copy_le_progress; auto; rew vec.
           { simpl; generalize (a*k); intro; omega. }
           do 3 f_equal; simpl mult; generalize (a*k); intro; omega.
         * apply IHa; rew vec.
           apply vec_pos_ext; intros y; dest y dst; try ring; dest y src.
     Qed.
 
-    Let mm2_mod_cst_spec_2 v w :
+    Let mma_mod_cst_spec_2 v w :
            0 < v#>src < k
         -> w = v[0/src][((v#>src)+(v#>dst))/dst]
-        -> (i,mm2_mod_cst) // (i,v) -+> (q,w).
+        -> (i,mma_mod_cst) // (i,v) -+> (q,w).
     Proof.
-      intros H ?; subst; unfold mm2_mod_cst.
+      intros H ?; subst; unfold mma_mod_cst.
       case_eq (v#>src).
       { intros; try omega. }
       intros x Hx.
-      mm2 sss DEC S with src (3+i) x.
-      mm2 sss INC with src.
-      apply subcode_sss_compute with (P := (4+i,mm2_decs_copy src dst i q k (4+i))); auto.
+      mma sss DEC S with src (3+i) x.
+      mma sss INC with src.
+      apply subcode_sss_compute with (P := (4+i,mma_decs_copy src dst i q k (4+i))); auto.
       { subcode_tac; rewrite <- app_nil_end; auto. }
-       apply sss_progress_compute, mm2_decs_copy_lt_progress; auto; rew vec; omega.
+       apply sss_progress_compute, mma_decs_copy_lt_progress; auto; rew vec; omega.
     Qed.
  
-    Fact mm2_mod_cst_divides_progress v a st :
+    Fact mma_mod_cst_divides_progress v a st :
             v#>src = a*k
          -> st = (p,v[0/src][((v#>src)+(v#>dst))/dst])
-         -> (i,mm2_mod_cst) // (i,v) -+> st.
+         -> (i,mma_mod_cst) // (i,v) -+> st.
     Proof.
       intros H1 ?; subst st.
       apply sss_compute_progress_trans with (i,v[0/src][((v#>src)+(v#>dst))/dst]).
-      + apply mm2_mod_cst_spec_1 with (a := a) (b := 0); try omega.
+      + apply mma_mod_cst_spec_1 with (a := a) (b := 0); try omega.
         rewrite <- H1; auto.
-      + apply mm2_mod_cst_spec_0; rew vec.
+      + apply mma_mod_cst_spec_0; rew vec.
     Qed.
 
-    Fact mm2_mod_cst_not_divides_progress v a b st :
+    Fact mma_mod_cst_not_divides_progress v a b st :
             v#>src = a*k+b
          -> 0 < b < k
          -> st = (q,v[0/src][((v#>src)+(v#>dst))/dst])
-         -> (i,mm2_mod_cst) // (i,v) -+> st.
+         -> (i,mma_mod_cst) // (i,v) -+> st.
     Proof.
       intros H1 H2 ?; subst st.
       apply sss_compute_progress_trans with (i,v[b/src][(a*k+(v#>dst))/dst]).
-      + apply mm2_mod_cst_spec_1 with (a := a) (b := b); try omega; auto.
-      + apply mm2_mod_cst_spec_2; rew vec.
+      + apply mma_mod_cst_spec_1 with (a := a) (b := b); try omega; auto.
+      + apply mma_mod_cst_spec_2; rew vec.
         apply vec_pos_ext; intros y; dest y dst; try omega; dest y src.
     Qed.
   
-  End mm2_mod_cst.
+  End mma_mod_cst.
 
-  Hint Rewrite mm2_decs_length mm2_mod_cst_length : length_db.
+  Hint Rewrite mma_decs_length mma_mod_cst_length : length_db.
 
-  Section mm2_div_cst.
+  Section mma_div_cst.
 
     (* Division by a constant *)
 
@@ -477,50 +477,49 @@ Section Minsky_Machine_alt_utils.
     Let p := (2+3*k+i).
     Let q := (5+3*k+i).
 
-    Definition mm2_div_cst := 
-         mm2_decs src p q k i ++ INC dst :: INC src :: DEC src i :: nil.
+    Definition mma_div_cst := 
+         mma_decs src p q k i ++ INC dst :: INC src :: DEC src i :: nil.
 
-    Fact mm2_div_cst_length : length mm2_div_cst = 5+3*k.
-    Proof. unfold mm2_div_cst; rew length; omega. Qed.
+    Fact mma_div_cst_length : length mma_div_cst = 5+3*k.
+    Proof. unfold mma_div_cst; rew length; omega. Qed.
 
     Hypothesis (Hk : 0 < k).
 
-    Let mm2_div_cst_spec a v w :
+    Let mma_div_cst_spec a v w :
            v#>src = a*k
         -> w = v[0/src][(a+(v#>dst))/dst]
-        -> (i, mm2_div_cst) // (i,v) -+> (q,w).
+        -> (i, mma_div_cst) // (i,v) -+> (q,w).
     Proof.
-      unfold mm2_div_cst; revert v w; induction a as [ | a IHa ]; intros v w H1 ?; subst w.
-      + apply subcode_sss_progress with (P := (i,mm2_decs src p q k i)); auto.
-        apply mm2_decs_lt_progress; try omega.
+      unfold mma_div_cst; revert v w; induction a as [ | a IHa ]; intros v w H1 ?; subst w.
+      + apply subcode_sss_progress with (P := (i,mma_decs src p q k i)); auto.
+        apply mma_decs_lt_progress; try omega.
         f_equal; simpl.
         apply vec_pos_ext; intros y; dest y dst.
       + apply sss_progress_trans with (p,v[(a*k)/src]).
-        * apply subcode_sss_progress with (P := (i,mm2_decs src p q k i)); auto.
-          apply mm2_decs_le_progress.
+        * apply subcode_sss_progress with (P := (i,mma_decs src p q k i)); auto.
+          apply mma_decs_le_progress.
           - rewrite H1; simpl; generalize (a*k); intro; omega.
           - f_equal.
             apply vec_pos_ext; intros y; dest y dst; dest y src.
             rewrite H1; simpl; generalize (a*k); intro; omega.
         * unfold p.
-          mm2 sss INC with dst.
-          mm2 sss INC with src.
-          mm2 sss DEC S with src i (a*k); rew vec.
+          mma sss INC with dst.
+          mma sss INC with src.
+          mma sss DEC S with src i (a*k); rew vec.
           apply sss_progress_compute, IHa; rew vec.
           apply vec_pos_ext; intros y; dest y dst; try omega; dest y src.
     Qed.
 
-    Fact mm2_div_cst_progress a v st :
+    Fact mma_div_cst_progress a v st :
             v#>src = a*k
          -> st = (q,v[0/src][(a+(v#>dst))/dst])
-         -> (i, mm2_div_cst) // (i,v) -+> st.
+         -> (i, mma_div_cst) // (i,v) -+> st.
     Proof.
-      intros H1 H2; subst st; apply mm2_div_cst_spec with (1 := H1); auto.
+      intros H1 H2; subst st; apply mma_div_cst_spec with (1 := H1); auto.
     Qed.
 
-  End mm2_div_cst.
+  End mma_div_cst.
 
-  Hint Rewrite mm2_div_cst_length : length_db.
+  Hint Rewrite mma_div_cst_length : length_db.
 
- 
 End Minsky_Machine_alt_utils.
